Update for today

MyMain.thy
@@ -8,15 +8,102 @@ lemma "\<forall> self caller om. eval (MyOCL.Eq (MyOCL.Var self) (MyOCL.Var call
 proof auto
 qed
 
+
+lemma lem1 : "\<forall> persons var. filterWhere (mapList persons) 
+(WHERE (MySQL.Eq (Col MySQL.ID) (MySQL.Var var)))
+= VList [extElement var persons]"
+  sorry
+
+fun equalVar :: "var \<Rightarrow> Person \<Rightarrow> bool" where
+"equalVar v (P pid page pemail pstudents plecturers) = (v = pid)"
+
+lemma lemSQL1 : "equalVar v p \<Longrightarrow> 
+extElement v (Cons p ps)
+ = VPerson p"
+  apply (induct p)
+  apply (auto)
+  done
+
+lemma lemSQL2 : "\<not>equalVar v p \<Longrightarrow> 
+extElement v (Cons p ps)
+= extElement v ps"
+  apply (induct p)
+  apply (auto)
+  done
+
+lemma lemSQL3 : "equalVar v p \<Longrightarrow> 
+ext v col (Cons p ps)
+= proj (Col col) (VPerson p)"
+  apply (induct p)
+  apply auto
+  done
+
+lemma lemSQL4 : "\<not>equalVar v p \<Longrightarrow> 
+ext v col (Cons p ps)
+= ext v col ps"
+apply (induct p)
+  apply auto
+  done
+
+lemma lem2 : "\<forall> col v. proj (Col col) (extElement v om) 
+= ext v col om"
+proof (induct om)
+  case Nil
+  then show ?case 
+    by simp
+next
+  case (Cons p ps)
+  then show ?case
+  proof (cases "equalVar v p")
+    case True
+    then show ?thesis 
+      using lemSQL1 lemSQL2 lemSQL3 lemSQL4 by metis
+  next
+    case False
+    then show ?thesis 
+      using lemSQL1 lemSQL2 lemSQL3 lemSQL4 by metis
+  qed
+qed
+ 
 (* self.age = 30 *)
 lemma "\<forall> om self. eval (MyOCL.Eq (MyOCL.Att self MyOCL.AGE) (MyOCL.Int 30)) om
 = exec (SelectFromWhere (MySQL.Eq (MySQL.Col (MySQL.AGE)) (MySQL.Int 30))
-(FROM table)
-(WHERE (MySQL.Eq (MySQL.Col (MySQL.ID)) (MySQL.Var self)))) om"
-proof auto
-qed
+(Table PERSON)
+(WHERE (MySQL.Eq (MySQL.Col (MySQL.ID)) (MySQL.Var self)))) om" 
+  apply auto
+   apply (simp_all add: lem1 lem2)
+  done
+
+lemma lem3 : "\<forall> persons var. filterWhere (mapList persons) 
+(WHERE (MySQL.Eq (Col MySQL.STUDENTS) (MySQL.Var var)))
+= VList [extElement var persons]"
+  sorry
+
+lemma singleVal : "val = VList [val]"
+  sorry
+
+(* self.lecturers *)
+lemma "eval (MyOCL.As self MyOCL.LECTURERS) om
+= exec (SelectFromWhere (MySQL.Col MySQL.LECTURERS) 
+(Table ENROLLMENT)
+(WHERE (MySQL.Eq (MySQL.Col (MySQL.STUDENTS)) (MySQL.Var self)))) om"
+  apply auto
+  apply(simp_all add: lem3 lem2 singleVal)
+  done
+
+(* self.lecturers\<rightarrow>size() *)
+lemma "eval (MyOCL.Size (MyOCL.As self MyOCL.LECTURERS)) om
+= exec (SelectFromWhere (MySQL.Count MySQL.LECTURERS) 
+(Table ENROLLMENT)
+(WHERE (MySQL.Eq (MySQL.Col (MySQL.STUDENTS)) (MySQL.Var self)))) om"
+   apply auto
+  apply(simp_all add: lem3 lem2)
+  done
+
+
 
 end
+
   
 
 
