ObjectModel.thy
@@ -4,20 +4,24 @@ begin
 
 (* Person(id, age, email, students, lecturers) *)
 datatype Person = P string int string "Person list" "Person list"
-(* Enrollment(students, lecturers) *)
-datatype Enrollment = E Person Person
 
 type_synonym persons = "Person list" 
 
-datatype val =  VInt int | VString string 
+datatype val =  VNULL | VInt int | VString string 
   |  VBool bool | VPerson Person | VList "val list"
 
 fun appList :: "val \<Rightarrow> val \<Rightarrow> val" where
-"appList v (VList vs) = VList (v#vs)"
+"appList v (VList vs) = VList (v#vs)" |
+"appList v VNULL = VNULL" |
+"appList _ _ = VNULL"
 
-fun mapList :: "Person list \<Rightarrow> val" where
+fun mapList :: "persons \<Rightarrow> val" where
 "mapList Nil = VList []" |
 "mapList (Cons p ps) = appList (VPerson p) (mapList ps)"
+
+fun isEmpty :: "val \<Rightarrow> bool" where 
+"isEmpty (VList Nil) = True" |
+"isEmpty _ = False"
 
 fun equalVal :: "val \<Rightarrow> val \<Rightarrow> bool" where
 "equalVal (VInt i1) (VInt i2) = (i1 = i2)" |
@@ -28,5 +32,9 @@ fun equalVal :: "val \<Rightarrow> val \<Rightarrow> bool" where
 "equalVal (VList (Cons v1 v1s)) (VList (Cons v2 v2s)) = 
 (if (equalVal v1 v2) then (equalVal (VList v1s) (VList v2s)) else False)" |
 "equalVal _ _ = False" 
+
+fun count :: "val \<Rightarrow> int" where 
+"count (VList Nil) = 0" |
+"count (VList (v#vs)) = 1 + count (VList vs)" 
 
 end
